Main.dfy
@@ -20,6 +20,7 @@ method Main(s : seq<string>)
   print "xxx", (s[1][0]), "xxx\n";
 
    match (s[1][0]) {
+     case '0' =>  Main0();
      case '1' =>  Main1();
      case '2' =>  Main2();
      case '3' =>  Main3();
@@ -30,6 +31,177 @@ method Main(s : seq<string>)
   print "Exit, pursued by a bear\n";
  }
 }
+
+method {:verify false} Main0() {
+
+  print "Main Test for loopback\n";
+
+var t := new Object.make(protoTypes, {}, {}, "t");
+
+//   t
+//   a      b c
+//   d
+//   e f g h
+
+assert t.Ready();
+assert COK(t, {t});
+
+// protoTypes 8-)
+// cat dat eye fucker jat kye lat nxt rat
+
+var a := new Object.make(protoTypes, {t}, {t}, "a");
+
+var b := new Object.make(protoTypes, {t}, {t}, "b");
+
+var c := new Object.make(protoTypes, {t}, {t}, "c");
+
+var d := new Object.make(protoTypes, {a}, {t,a}, "d");
+
+var e := new Object.make(protoTypes, {d}, {t,a,d}, "e"); //we're gonna clone this one..?
+
+var f := new Object.make(protoTypes, {e}, {t,a,d,e}, "f");
+
+var g := new Object.make(protoTypes, {f},  {t,a,d,e,f},   "g");
+
+var h := new Object.make(protoTypes, {g}, {t,a,d,e,f,g}, "h");
+
+
+var i := new Object.make(protoTypes, {e}, {t,a,d,e,f,g,h}, "i");
+var j := new Object.make(protoTypes, {e}, {t,a,d,e,f,g,h}, "j");
+var k := new Object.make(protoTypes, {e}, {t,a,d,e,f,g,h}, "k");
+var l := new Object.make(protoTypes, {e}, {t,a,d,e,f,g,h}, "l");
+
+
+assert t.Ready();
+
+assert a.Ready();
+assert b.Ready();
+assert c.Ready();
+assert d.Ready();
+assert e.Ready();
+assert f.Ready();
+assert g.Ready();
+assert h.Ready();
+assert i.Ready();
+assert j.Ready();
+assert k.Ready();
+assert l.Ready();
+
+var os : set<Object> := {t,   a, b, c, d, e, f, g, h, i, j, k, l};
+
+print "|os| == ", |os|, "\n";
+
+a.fields := map["eye":=d];
+d.fields := map["lat":= e]["dat":=f]["cat":=g]["rat":= h];
+
+assert COK(a,os);
+
+assert d.AllFieldsAreDeclared();
+assert d.AllFieldsContentsConsistentWithTheirDeclaration();
+assert d.AllOutgoingReferencesAreOwnership(os);
+assert d.AllOutgoingReferencesWithinThisHeap(os);
+assert COK(d,os);
+
+
+assert CallOK(os);
+
+print "+++++++++++++\n";
+print "original store (os)\n";
+print "+++++++++++++\n";
+printobjectset(os);
+print "+++++++++++++\n";
+
+print "done setup\n";
+
+// printobj(a);
+// printobjfields(a);
+
+// print "here edgeset\n";
+assert forall o <- os :: o.Ready();
+// printedgeset(edges(os));
+// print "done edgeset\n\n";
+
+// printobj(d); printobjfields(d);
+// printobj(e); printobjfields(e);
+
+// print d.region,"\n";
+// print e.region,"\n";
+
+// assert !d.region.World?;
+// assert !e.region.World?;
+
+//assert isIsomorphicMappingOWNED(d, d, isomap, os);
+
+// print "ISO ISO ISO\n";
+
+// var ros := walkies(d, d, isomap, os);
+
+// return;
+
+print "%%%%%%%%%%%%%%%%%%%%%%%%%%%%%%%%%%%%%%%%%%%%%%%%%%%%%%%%%%%%%%\n";
+
+//////reveal Object.Ready();
+assert t.AllOwnersAreWithinThisHeap(os);
+assert a.AllOwnersAreWithinThisHeap(os);
+assert b.AllOwnersAreWithinThisHeap(os);
+assert c.AllOwnersAreWithinThisHeap(os);
+assert d.AllOwnersAreWithinThisHeap(os);
+assert e.AllOwnersAreWithinThisHeap(os);
+assert f.AllOwnersAreWithinThisHeap(os);
+assert g.AllOwnersAreWithinThisHeap(os);
+assert h.AllOwnersAreWithinThisHeap(os);
+assert i.AllOwnersAreWithinThisHeap(os);
+assert j.AllOwnersAreWithinThisHeap(os);
+assert k.AllOwnersAreWithinThisHeap(os);
+assert l.AllOwnersAreWithinThisHeap(os);
+
+assert forall o <- os :: (o.AllOwnersAreWithinThisHeap(os));
+
+print "about to Xlone a\n";
+
+
+var m := Klon(map[],    //m clonemap
+               a,       // o - object to be cloned / pivot / top object
+               a.AMFO,  // o_amfo AMFO of o
+               a.owner,  // c_owner - proposewd owner of clone
+               a.AMFX,   // c_amfx - AMFX of clone
+               os,      // oHeap
+               {}       // ns;
+              );
+
+var ra, rm := Xlone_Via_Map(a, m);
+
+// //
+// //     m : Mapping,  //m : Mapping
+// //     ks : set<Object>, //ks - set, keys of the mapping   (must be m.Keys, subset of oHeap)
+// //     vs : set<Object>, //vs - set, values or the mapping (must be m.Values, subset of oHeap + ns)
+// //     o : Object,  //o - Owner within which the clone is being performaed, in oHeap
+// //     oHeap : set<Object>,  //oHeap - original (sub)heap contianing the object being cloned and all owners and parts
+// //     ns : set<Object>)
+
+print "+++++++++++++\n";
+print "original store (os)\n";
+print "+++++++++++++\n";
+printobjectset(os);
+print "+++++++++++++\n";
+print "clones rm.Values - os\n";
+print "+++++++++++++\n";
+printobjectset(rm.m.Values - os);
+print "+++++++++++++\n";
+printmapping(rm.m);
+
+print "\n\n\n\nwaiting...\\n\n";
+
+var result : bool :=  istEinKlon(a, rm, (os + rm.m.Values + rm.ns));
+print "istEinKlon = ", result;
+
+print "\n\n";
+
+print "\nDone\n";
+}
+// end
+
+
 
 method {:verify false} Main1() {
 
@@ -88,6 +260,9 @@ assert l.Ready();
 
 var os : set<Object> := {t,   a, b, c, d, e, f, g, h, i, j, k, l};
 
+print "|os| == ", |os|, "\n";
+
+
 a.fields := map["eye":=d];
 d.fields := map["lat":= e]["dat":=f]["cat":=g]["rat":= h];
 
@@ -101,6 +276,12 @@ assert COK(d,os);
 
 
 assert CallOK(os);
+
+print "+++++++++++++\n";
+print "original store (os)\n";
+print "+++++++++++++\n";
+printobjectset(os);
+print "+++++++++++++\n";
 
 print "done setup\n";
 
@@ -148,11 +329,20 @@ assert l.AllOwnersAreWithinThisHeap(os);
 
 assert forall o <- os :: (o.AllOwnersAreWithinThisHeap(os));
 
-print "about to clone a\n";
+print "about to Clone a\n";
 
-var m := Klon(map[], a, a.AMFO, a.AMFO, os, {}, {} );
+var m := Klon(map[],    //m clonemap
+               a,       // o - object to be cloned / pivot / top object
+               a.AMFO,  // o_amfo AMFO of o
+               a.owner,  // c_owner - proposewd owner of clone
+               a.AMFX,   // c_amfx - AMFX of clone
+               os,      // oHeap
+               {}       // ns );
+              );
 
 var ra, rm := Clone_Via_Map(a, m);
+
+
 
 // //
 // //     m : Mapping,  //m : Mapping
@@ -183,8 +373,6 @@ print "\n\n";
 print "\nDone\n";
 }
 // end
-
-
 
 
 
