X2.dfy
@@ -1,0 +1,312 @@
+//Xlone_Via_Map -> Xlone_Xlone_Clone
+//Xlone_Xlone_xClone -> Xlone_All_Owners, Object.make(), putInside/putOutside, Xlone_All_Fields
+//Xlone_All_Owners -> Xlone_Via_Map
+//Xlone_All_Fields -> Xlone_Field_Map
+//Xlone_Field_Map ->  Xlone_Via_Map
+
+method Xlone_Via_Map(a : Object, m' : Klon)
+  returns (b : Object, m : Klon)
+  decreases |m'.oHeap - m'.m.Keys|, |a.AMFO|, |a.fields.Keys|, 20 //Klone_Via_Map
+
+{
+  m := m';
+
+  print "CALL Clone_Via_Map ", fmtobj(a), "\n";
+
+  print "VARIANT CVM ", |(m'.oHeap - m'.m.Keys)|, " ", |a.AMFO|, " ", |(a.fields.Keys )|, " ", 20, "\n";
+
+  if (a in m.m.Keys){ //already cloned, return
+    b := m.m[a];
+    print "RETN Clone_Via_Map already cloned ", fmtobj(a), "\n";
+    return;
+  }
+
+  if (outside(a,m.o)) { //outside. so just map to itself
+    b := a;
+    m := m.putOutside(a);
+    print "RETN Clone_Via_Map: outside ", fmtobj(a), "\n";
+    return; // end outside case
+  }
+
+  b, m := Xlone_Clone_Clone(a, m);
+  //end of inside case
+
+  print "RETN Clone_Via_Map: ", fmtobj(a), " pivot:", fmtobj(m.o), "\n";
+
+}//END Xlone_Via_Map
+
+
+
+
+
+
+method Xlone_Clone_Clone(a : Object, m' : Klon)
+  returns (b : Object, m : Klon)
+    decreases |m'.oHeap - m'.m.Keys|, |a.AMFO|, |a.fields.Keys|, 15
+{
+  m := m';
+
+  print "CALL Clone_Clone_CLone of:", fmtobj(a), " owned by ", fmtown(a.owner) ,"\n";
+  print "VARIANT CCC ", |(m'.oHeap - m'.m.Keys)|, " ", |a.AMFO|, " ", |(a.fields.Keys)|, " ", 15, "\n";
+
+  print "Clone_Clone_Clone ", fmtobj(a), " calling CAO", fmtown(a.owner) ,"\n";
+  printmapping(m.m);
+
+/////////////////////////////////////////////////////////////////////////////////
+  var rm := Xlone_All_Owners(a, m);
+/////////////////////////////////////////////////////////////////////////////////
+
+ var rowner := a.owner;
+ var rbound := a.bound;
+
+  var rAMXO := flattenAMFOs(rowner);
+  var rAMXB := flattenAMFOs(rbound);
+
+
+  if (a in rm.m.Keys) {
+
+    m := rm;
+    b := m.XXXat(a); //HMM
+
+//END FUCKOFF
+    print "RETN Clone_Clone_CLone ", fmtobj(a), " already cloned: abandoning ship!!\n";
+    return;
+  } // a in rm.m.Keys - i.e. randomly done while cloning owners
+
+
+  print "Clone_Clone_CLone ", fmtobj(a), " have rowner ", fmtown(rowner) ," self not yet cloned\n";
+
+var rrm := rm; //KJX THIS IS EVIL, should clean up and get rid of rrm completel6.
+
+
+print "Clone_Clone_Clone ", fmtobj(a), " boodle boodle boodle\n";
+
+
+  var context := rrm.oHeap+rrm.ns;    ///why haul ns in here??? --- cos this the owners for the clone!  - the clowners!
+
+
+print "CALLING MAKE...";
+
+  b := new Object.XXXmake(a.fieldModes, rowner, rrm.oHeap+rrm.ns, "clone of " + a.nick, rbound);
+print "BACK FROM MAKE with ",fmtobj(b),"\n";
+
+
+  //  var km := klonKV(rrm,a,b); //there it go4s in!
+
+  var km := rrm.(ns := rrm.ns + nu(a,b)).(m:= VMapKV(rrm.m,a,b));
+
+var amxo := flattenAMFOs(a.owner);
+
+  var xm := rrm.putInside(a,b);
+
+  print "Clone_Clone_Clone map updated ", fmtobj(a), ":=", fmtobj(b) ,"\n";
+
+   m := Xlone_All_Fields(a,b, xm);
+
+  print "RETN Clone_Clone_CLone of ", fmtobj(a), " retuning ", fmtobj(b) ,"\n";
+
+  assert m.m.Values >= m'.m.Values + {b};
+}//end Clone_Clone_Clone
+
+
+
+
+
+
+
+
+
+
+
+
+
+
+
+
+
+
+//$$$$$$$$$$$$$$$$$$$$$$$$$$$$$$$$$$$$$$$$$$$$$$$$$$$$$$$$$$$$$$$$$$$$$$$$$$$$$
+
+
+
+
+
+
+ method Xlone_All_Owners(a : Object,  m' : Klon)  returns (m : Klon)
+  //decreases |m'.oHeap| - |m'.m.Keys| + |{a}|, |a.AMFO|, |a.fields.Keys|, 12
+  decreases |m'.oHeap - m'.m.Keys|, |a.AMFO|, |a.fields.Keys|, 12
+
+{
+  print "CALL Clone_All_Owner of:", fmtobj(a), " owned by ", fmtown(a.owner) ,"\n";
+  print "VARIANT CAO ", |(m'.oHeap - m'.m.Keys)|, " ", |a.AMFO|, " ", |(a.fields.Keys)|, " ", 12, "\n";
+  print "ENTRY   CAO ", a.owner - m'.m.Keys ," a in Keys ", (a !in m'.m.Keys), "\n";
+
+  var rm := m';
+  var b : Object;  //do we care..
+
+  var xm := rm;
+
+  var xo : Object;
+  var rr : Object;
+  var oldmks  : set<Object>;  //dont fucking ask
+  var oldmok :=  false;
+
+  var MX := a.owner - xm.m.Keys;
+
+     print "PRELOOP ", |MX|," a in Keys ", (a !in xm.m.Keys), "\n";
+
+  while ((MX != {}) && (a !in xm.m.Keys))
+
+  {
+
+      print "LOOPTOP ", |MX|," a in Keys ", (a !in xm.m.Keys), "\n";
+
+    xo :| xo in MX;
+
+    MX := MX - {xo};
+
+    rr, rm := Xlone_Via_Map(xo, xm);
+
+
+    if (a in rm.m.Keys) {
+      m := rm;
+      b := m.m[a];
+
+      print "RETN - Clone All Onwers - already clonéd\n";
+      return;
+    }  // if a is in m.Keys after clone -- if it got added magically...
+
+
+    MX := MX - rm.m.Keys;
+
+    oldmks := xm.m.Keys;
+    oldmok := true;
+    xm := rm;
+  } // end loop MX
+
+  m := xm;
+
+      print "RETN - Clone All Onwers - done Done DONE\n";
+
+}//END Xlone_All_Owners
+
+
+
+
+
+
+
+
+
+
+
+
+
+
+
+method Xlone_All_Fields(a : Object, b : Object, m' : Klon)
+  returns (m : Klon)
+
+  decreases |m'.oHeap - m'.m.Keys|, |a.AMFO|, fielddiff(a,b), 10
+
+  modifies b`fields
+{
+  print "CALL Clone_All_Fields: ", fmtobj(a), " pivot:", fmtobj(m'.o), "\n";
+
+  m := m';
+
+//TUESDAY15DEC2024
+
+  print "VARIANT CAF ", |(m'.oHeap - m'.m.Keys)|, " ", |a.AMFO|, " ", |(a.fields.Keys)|, " ", 10, "\n";
+  print "<<<<<<<<<<<\n";
+  print "just cloned ", fmtobj(a), " as ", fmtobj(b), "\n";
+  print "<<<<<<<<<<<\n";
+
+
+  print "<<<<<<<<<<<\n";
+  printmapping(m.m);
+  print "<<<<<<<<<<<\n";
+
+  var fieldNames : seq<string> := set2seq(a.fields.Keys);
+
+
+ print "Clone_All_Fields fields:", fmtobj(a), " fields=", fmtseqstr(fieldNames), "\n";
+
+
+  print "BLOOP BLOOP BLOOP\n";
+  var rm := m;
+
+  for i := 0 to |fieldNames|
+
+  {
+    var n : string := fieldNames[i];
+    var ofv : Object := a.fields[n];
+
+    print "  TLOOP  ",fmtobj(a),".",n," :=", fmtobj(ofv), "\n";
+    print "  TLOOP  (recurse on field ",n,")\n";
+    print "  TLOOP m:", |m.oHeap - m.m.Keys|, " m':", |m'.oHeap - m'.m.Keys|, "\n";
+    print "  TLOOP b.fieldsKeys==", b.fields.Keys, "\n";
+    print "  TINV                ", fieldNames[..i], "\n";
+    print "  TLOOPINV            ",seq2set(fieldNames[..i]),"\n";
+
+    print "VARIANT*CAF ", |(m'.oHeap - m'.m.Keys)|, " ", |a.AMFO|, " ", |(a.fields.Keys)|, " ", 10, "\n";
+
+    var OLDFLDS := b.fields.Keys;
+
+    var v_caf := ((m'.oHeap - m'.m.Keys +{a}), a.AMFO, (a.fields.Keys), 10);
+    var v_cfm := ((m.oHeap - m.m.Keys +{a}), a.AMFO, (a.fields.Keys - b.fields.Keys), 5);//Xlone_Field_Map
+
+    print "v_caf ", v_caf, "\n";
+    print "v_cfm ", v_cfm, "\n";
+
+    print "okaoka ", (m'.oHeap - m'.m.Keys +{a}) >  (m.oHeap - m.m.Keys +{a}), "\n";
+    print "okaoka ", (m'.oHeap - m'.m.Keys +{a}) == (m.oHeap - m.m.Keys +{a}), "\n";
+
+print "WHOOPS-> ", |m'.oHeap - m'.m.Keys +{a}|, " ", |a.AMFO|," ",|a.fields.Keys - b.fields.Keys|," 10\n";
+print "->WHOOPS ", |m'.oHeap - m'.m.Keys +{a}|, " ", |a.AMFO|," ",|a.fields.Keys - b.fields.Keys|," 5 \n";
+
+    rm := Xlone_Field_Map(a,n,b,m);
+  }
+
+  print "RETN Clone_All_Fields done ", fmtobj(a), "\n";
+
+  return;
+}
+//end Xlone_All_Fields
+
+
+
+
+
+
+method Xlone_Field_Map(a : Object, n : string, b : Object, m' : Klon)
+  returns (m : Klon)
+
+  decreases |m'.oHeap - m'.m.Keys|, |a.AMFO|, fielddiff(a,b), 5 //Xlone_Field_Map
+
+  modifies b`fields
+{
+
+  print "CALL Clone_Field_Map ", fmtobj(a), " «", n, "»\n";
+  print "VARIANT CFM ", |m'.oHeap - m'.m.Keys|, " ", |a.AMFO|, " ", fielddiff(a,b), " ", 5, "\n";
+
+  m := m';
+
+  var v_cfm := ((m.oHeap - m.m.Keys), a.AMFO, (a.fields.Keys - b.fields.Keys), 5);//Xlone_Field_Map *variant for decreases clause*
+
+  var onb := m.ns - {b};
+  var ctx := (m.oHeap+m.ns);
+
+  var ofv := XXXCOKat(a,n,m.oHeap);
+
+  // // // // // // // // // // // // // // // // // // // // // // // // // // // // // // // // //
+  var rfv, rm := Xlone_Via_Map(ofv, m);
+  // // // // // // // // // // // // // // // // // // // // // // // // // // // // // // // // //
+
+  m.XXXCOKput(b, m.oHeap+m.ns, n, rfv);
+
+  // // // // // // // // // // // // // // // // // // // // // // // // // // // // // // // // //
+
+  print "RETN Clone_Field_Map: ", fmtobj(a), " pivot:", fmtobj(m.o), "\n";
+
+} //end Clone: /_Field_Map
